## Fundamental Laws
                    
<div class="law-box">
    <h5>1. Identity Laws</h5>
    <div class="boolean-algebra">
A + 0 = A    (OR with 0 doesn't change A)
A · 1 = A    (AND with 1 doesn't change A)
                        </div>
                    </div>
                    
<div class="law-box">
                        <h5>2. Null (Domination) Laws</h5>
                        <div class="boolean-algebra">
A + 1 = 1    (OR with 1 is always 1)
A · 0 = 0    (AND with 0 is always 0)
                        </div>
                    </div>
                    
<div class="law-box">
                        <h5>3. Idempotent Laws</h5>
                        <div class="boolean-algebra">
A + A = A    (ORing with itself gives same value)
A · A = A    (ANDing with itself gives same value)
                        </div>
                    </div>
                    
<div class="law-box">
                        <h5>4. Complement Laws</h5>
                        <div class="boolean-algebra">
A + A' = 1   (A OR NOT A is always TRUE)
A · A' = 0   (A AND NOT A is always FALSE)
(A')' = A    (Double negation returns original)
                        </div>
                    </div>
                    
<div class="law-box">
                        <h5>5. Commutative Laws</h5>
                        <div class="boolean-algebra">
A + B = B + A    (Order doesn't matter in OR)
A · B = B · A    (Order doesn't matter in AND)
                        </div>
                    </div>
                    
<div class="law-box">
                        <h5>6. Associative Laws</h5>
                        <div class="boolean-algebra">
A + (B + C) = (A + B) + C    (Grouping doesn't matter in OR)
A · (B · C) = (A · B) · C    (Grouping doesn't matter in AND)
                        </div>
                    </div>
                    
<div class="law-box">
                        <h5>7. Distributive Laws</h5>
                        <div class="boolean-algebra">
A · (B + C) = (A · B) + (A · C)    (AND distributes over OR)
A + (B · C) = (A + B) · (A + C)    (OR distributes over AND)
                        </div>
                    </div>
                    
<div class="law-box">
                        <h5>8. Absorption Laws</h5>
                        <div class="boolean-algebra">
A + (A · B) = A    (Absorbs the AND term)
A · (A + B) = A    (Absorbs the OR term)
                        </div>
                    </div>